src/lib/kuiper/Kuiper.Common.fsti
@@ -14,6 +14,7 @@ type natlt (b:int) = n:nat{n <  b}
 type natle (b:int) = n:nat{n <= b}
 type posmultiple (k:int) = n:pos{k /? n}
 
+type binop (t : Type) = t -> t -> t
 
 (* Erased version, with refinement **on the outside** to prevent
 against invariance of erased wrt types. *)
