src/lib/poly/gemm/Kuiper.Poly.GEMM.Tiled.fsti
@@ -6,4 +6,4 @@ open Kuiper
 open Kuiper.Poly.GEMMGPU.Type
 
 inline_for_extraction noextract
-val matmul_gpu : tiled_matmul_gpu_ty
+val matmul_gpu : tiled_matmulcomb_gpu_ty
